ConZF.lean
@@ -1,3 +1,7 @@
 import ConZF.PSet
 import ConZF.Mat
 import ConZF.Repl
+import ConZF.Rule
+import ConZF.Pair
+import ConZF.Ord
+import ConZF.VLevel
